WIP

hol/p4_exec_semSyntax.sig
@@ -7,4 +7,9 @@ val dest_arch_multi_exec : term -> term * term * term
 val is_arch_multi_exec : term -> bool
 val mk_arch_multi_exec : term * term * int -> term
 
+val red_seq_empty_tm : term
+val dest_red_seq_empty : term -> term
+val is_red_seq_empty : term -> bool
+val mk_red_seq_empty : term -> term
+
 end
