hol/p4_exec_semSyntax.sml
@@ -11,4 +11,7 @@ val (arch_multi_exec_tm, _, dest_arch_multi_exec, is_arch_multi_exec) =
 val mk_arch_multi_exec =
  (fn (ctx, state, fuel) => (#2 (syntax_fns3 "p4_exec_sem" "arch_multi_exec")) (ctx, state, term_of_int fuel));
 
+val (red_seq_empty_tm, mk_red_seq_empty, dest_red_seq_empty, is_red_seq_empty) =
+  syntax_fns1 "p4_exec_sem" "red_seq_empty";
+
 end
